git/cruhland/lean4-axiomatic/Lean4Axiomatic/Eqv.lean
@@ -7,8 +7,18 @@ namespace Relation
 class Swap {α : Sort u} {β : Sort v} (rα : α → α → β) (rβ : β → β → Prop) where
   swap : {x y : α} → rβ (rα x y) (rα y x)
 
+export Swap (swap)
+
+instance
+    {α : Sort u} {rel : α → α → Prop} [inst : Swap rel (· → ·)]
+    : Swap rel (· ↔ ·)
+    where
+  swap := ⟨swap (self := inst), swap (self := inst)⟩
+
 class Refl {α : Sort u} (rel : α → α → Prop) where
   refl : {x : α} → rel x x
+
+export Refl (refl)
 
 instance : Refl (· → ·) where
   refl := id
@@ -16,11 +26,15 @@ instance : Refl (· → ·) where
 class Symm {α : Sort u} (rel : α → α → Prop) where
   symm : {x y : α} → rel x y → rel y x
 
+export Symm (symm)
+
 instance {α : Sort u} {rel : α → α → Prop} [Symm rel] : Swap rel (· → ·) where
-  swap := Symm.symm
+  swap := symm
 
 class Trans {α : Sort u} (rel : α → α → Prop) where
   trans : {x y z : α} → rel x y → rel y z → rel x z
+
+export Trans (trans)
 
 instance : Trans (· → ·) where
   trans := λ f g x => g (f x)
@@ -42,19 +56,22 @@ class EqvOp? (α : Sort u)
 
 end Relation
 
+instance iff_symm : Relation.Symm (· ↔ ·) where
+  symm {p q : Prop} := by
+    intro ⟨(_ : p → q), (_ : q → p)⟩
+    show q ↔ p
+    exact ⟨‹q → p›, ‹p → q›⟩
+
 instance {α : Sort u} [Relation.EqvOp α] : Relation.Symm (α := α) (· ≄ ·) where
   symm := Relation.neq.symm
 
 instance
     {α : Sort u} {rel : α → α → Prop} [Relation.Trans rel]
     : Trans rel rel rel where
-  trans := Relation.Trans.trans
+  trans := Relation.trans
 
 namespace Eqv
 
-export Relation.Swap (swap)
-export Relation.Refl (refl)
-export Relation.Symm (symm)
-export Relation.Trans (trans)
+export Relation (refl swap symm trans)
 
 end Eqv
