git/leanprover/lean4/src/Init/Notation.lean
@@ -348,8 +348,8 @@ macro "try " t:tacticSeq : tactic => `(first | $t | skip)
 /-- `tac <;> tac'` runs `tac` on the main goal and `tac'` on each produced goal, concatenating all goals produced by `tac'`. -/
 macro:1 x:tactic " <;> " y:tactic:0 : tactic => `(tactic| focus ($x:tactic; all_goals $y:tactic))
 
-/-- `rfl` is a shorthand for `exact rfl`. -/
-macro "rfl" : tactic => `(exact rfl)
+/-- `rfl` is equivalent to `exact rfl`, but has a few optimizatons. -/
+syntax (name := refl) "rfl" : tactic
 
 /--
   Similar to `rfl`, but disables smart unfolding and unfolds all kinds of definitions,
